PDS/PDS_Code.thy
@@ -4,12 +4,16 @@ begin
 
 (*derive linorder operation*)
 
-global_interpretation pds: PDS_with_P_automaton \<Delta> "{f \<in> F_states. \<not> is_Ctr_Ext f}"
+
+global_interpretation pds: PDS_with_P_automaton \<Delta> F_ctr_loc F_ctr_loc_st
   for \<Delta> :: "('ctr_loc::{finite, linorder}, 'label::{finite, linorder}) rule set"
-  and F_states :: "('ctr_loc, 'state::{finite, linorder}, 'label) state set"
+  and F_ctr_loc :: "('ctr_loc) set"
+  and F_ctr_loc_st :: "('state::finite) set"
   defines pre_star = "PDS_with_P_automaton.pre_star_exec \<Delta>"
-  and accepts = "PDS_with_P_automaton.accepts {f \<in> F_states. \<not> is_Ctr_Ext f}"
-  by standard auto
+  and pre_star_check = "PDS_with_P_automaton.pre_star_exec_check \<Delta>"
+  and accepts = "PDS_with_P_automaton.accepts F_ctr_loc F_ctr_loc_st"
+  and accepts_pre_star_check = "PDS_with_P_automaton.accept_pre_star_exec_check \<Delta> F_ctr_loc F_ctr_loc_st"
+  .
 
 export_code pre_star in SML
 
@@ -45,11 +49,30 @@ definition \<P> :: "((ctr_loc, state, label) PDS.state, label) transition set" w
 
 value "pre_star \<Delta> \<P>"
 
+thm pds.theorem_3_2_exec_check
+
+value "pre_star_check \<Delta> \<P>"
+
+thm pds.theorem_3_2_exec
+
 value "(Ctr_Loc p0, [\<gamma>0, \<gamma>0], Ctr_Loc_St s2) \<in> LTS.transition_star (pre_star \<Delta> \<P>)" \<comment> \<open>True\<close>
 value "(Ctr_Loc p0, [\<gamma>0, \<gamma>1], Ctr_Loc_St s2) \<in> LTS.transition_star (pre_star \<Delta> \<P>)" \<comment> \<open>False\<close>
-value "accepts {Ctr_Loc_St s2} (pre_star \<Delta> \<P>) (p0, [\<gamma>0, \<gamma>0])" \<comment> \<open>True\<close>
-value "accepts {Ctr_Loc_St s1} (pre_star \<Delta> \<P>) (p0, [\<gamma>0, \<gamma>0])" \<comment> \<open>False\<close>
-value "accepts {Ctr_Loc_St s2} (pre_star \<Delta> \<P>) (p0, [\<gamma>0, \<gamma>1])" \<comment> \<open>False\<close>
+value "accepts {} {s2} (pre_star \<Delta> \<P>) (p0, [\<gamma>0, \<gamma>0])" \<comment> \<open>True\<close>
+value "accepts {} {s1} (pre_star \<Delta> \<P>) (p0, [\<gamma>0, \<gamma>0])" \<comment> \<open>False\<close>
+value "accepts {} {s2} (pre_star \<Delta> \<P>) (p0, [\<gamma>0, \<gamma>1])" \<comment> \<open>False\<close>
+
+thm pds.accept_pre_star_correct_True
+thm pds.accept_pre_star_correct_False
+
+value "accepts_pre_star_check \<Delta> {} {s2} \<P> (p0, [\<gamma>0, \<gamma>0])" \<comment> \<open>Some True\<close>
+value "accepts_pre_star_check \<Delta> {} {s1} \<P> (p0, [\<gamma>0, \<gamma>0])" \<comment> \<open>Some False\<close>
+value "accepts_pre_star_check \<Delta> {} {s2} \<P> (p0, [\<gamma>0, \<gamma>1])" \<comment> \<open>None\<close>
+
+thm pds.accept_pre_star_correct_Some_True
+thm pds.accept_pre_star_correct_Some_False
+thm pds.accept_pre_star_correct_None
+
+find_theorems accepts
 
 (*
 datatype ctr_loc = q
